\documentclass[10pt,a4paper]{article}
\usepackage[utf8]{inputenc}
\usepackage[a4paper,%
            left=.75in,right=.75in,top=1in,bottom=1in]{geometry}
\setlength{\headsep}{0.25in}

\usepackage{amsthm}

\usepackage{graphicx}
\usepackage{pgfplots}

\usepackage{hyperref}

\hypersetup{colorlinks=true, linkcolor=blue, urlcolor=cyan}
            
\usepackage[english]{babel}

\theoremstyle{theorem}
\newtheorem{theorem}{Theorem}
\newtheorem{lemma}{Lemma}
\newtheorem{corollary}{Corollary}
\newtheorem{case}{Case}

\newcommand\restr[2]{{% we make the whole thing an ordinary symbol
  \left.\kern-\nulldelimiterspace % automatically resize the bar with \right
  #1 % the function
  \vphantom{\big|} % pretend it's a little taller at normal size
  \right|_{#2} % this is the delimiter
  }}

\theoremstyle{definition}
\newtheorem{definition}{Definition}
\newtheorem{remark}{Remark}

\usepackage{mathtools}
\DeclarePairedDelimiter\bra{\langle}{\rvert}
\DeclarePairedDelimiter\ket{\lvert}{\rangle}
\DeclarePairedDelimiterX\braket[2]{\langle}{\rangle}{#1 \delimsize\vert #2}

\usepackage{amsmath}
\usepackage{amsfonts}
\usepackage{amssymb}
\usepackage{fancyhdr}

\DeclareMathOperator{\interior}{int}

\newcommand{\Tau}{\mathcal{T}}

\newcommand{\Prob}{\mathbb{P}}

\newenvironment{amatrix}[1]{%
  \left(\begin{array}{@{}*{#1}{c}|c@{}}
}{%
  \end{array}\right)
}

\usepackage{calligra}
\DeclareMathAlphabet{\mathcalligra}{T1}{calligra}{m}{n}
\DeclareFontShape{T1}{calligra}{m}{n}{<->s*[2.2]callig15}{}

\newcommand{\scripty}[1]{\ensuremath{\mathcalligra{#1}}}

\pagestyle{fancy}
\author{Jeremiah Givens}
\newcommand{\subject}{Probability MA 585}
\newcommand{\Date}{9/2/2021} 
\makeatletter
\rhead{{\small\@author}}
\lhead{{\small\subject}}
\chead{{\large Homework 2}}
\cfoot{}
\rfoot{\thepage}
\lfoot{\today}

\renewcommand{\theequation}{\arabic{equation}}

\begin{document}
\section*{Problem 2.8}
The density function of the two-dimensional random variable $(X, Y)$ is
\begin{align*}
f_{X, Y}(x, y) &= \begin{cases} 
      \frac{x^2}{2 y^3} e^{- \frac{x}{y}} & 0 \leq x \leq \infty, \text{ and } 0 \leq y \leq 1 \\
      0 & \text{otherwise.}
   \end{cases}
\end{align*}
\begin{enumerate}
\item[(a)] Determine the distribution of $Y$.
\item[(b)] Find the conditional distribution of $X$ given that $Y = y$.
\item[(c)] Use the results from (a) and (b) to compute $EX$ and $\text{Var}X$
\end{enumerate}

\subsection*{Solution}
\begin{enumerate}
\item[(a)] For $0 \leq y \leq 1$, we have
\begin{align*}
f_Y(y) &= \int_{-\infty}^{\infty} f_{X, Y}(x, y) dx\\
&= \int_{0}^{\infty} \frac{x^2}{2 y^3} e^{- \frac{x}{y}} dx\\
&= \frac{1}{2 y^3} \left( \int_{0}^{\infty} \left(\frac{\partial}{\partial x} (-yx^2 e^{- \frac{x}{y}}) + 2xy e^{- \frac{x}{y}}\right) dx \right)\\
&= \frac{1}{y^2} \int_{0}^{\infty} x e^{- \frac{x}{y}} dx\\
&= \frac{1}{y} \int_{0}^{\infty} e^{- \frac{x}{y}} dx\\
&= \left. - e^{- \frac{x}{y}} \right|_{0}^\infty\\
&= \boxed{1}.
\end{align*}

\item[(b)] From the definition of conditional distributions, we have
\begin{align*}
f_{X|Y = y}(x) &= \frac{f_{X, Y}(x, y)}{f_Y(y)}\\
&= \frac{f_{X, Y}(x, y)}{f_Y(y)}\\
&= f_{X, Y}(x, y)\\
&= \boxed{\begin{cases} 
      \frac{x^2}{2 y^3} e^{- \frac{x}{y}} & 0 \leq x \leq \infty, \text{ and } 0 \leq y \leq 1 \\
      0 & \text{otherwise.}
   \end{cases}}
\end{align*}

\item[(c)] 
\begin{align*}
EX &= \int_0^1 \int_0^\infty x f_{X, Y}(x, y) dx dy\\
&= \int_0^1 \int_0^\infty \frac{x^3}{2 y^3} e^{- \frac{x}{y}} dx dy\\
&= \boxed{\frac{3}{2}} && \text{after integration by parts 3 times}\\
EX^2 &= \int_0^1 \int_0^\infty x^2 f_{X, Y}(x, y) dx dy\\
&= \int_0^1 \int_0^\infty \frac{x^4}{2 y^3} e^{- \frac{x}{y}} dx dy\\ 
&= 4\\
\text{Var}X &= EX^2 - (EX)^2\\
&= 4 - (\frac{3}{2})^2\\
&= \frac{16 - 9}{4}\\
&= \boxed{\frac{7}{4}}
\end{align*}
\end{enumerate}

\section*{Problem 2.9}
The density of a random vector $(X, Y)'$ is 
\begin{align*}
f_{X, Y}(x, y) &= \begin{cases} 
      cx & x \geq 0, \text{ and } y \geq 0, \text{ and } x + y \leq 1 \\
      0 & \text{otherwise.}
   \end{cases}
\end{align*}
Compute 
\begin{enumerate}
\item[(a)] c,
\item[(b)] the conditional expectations $E(Y | X = x)$ and $E(X| Y = y)$.
\end{enumerate}

\subsection*{Solution}
\begin{enumerate}
\item[(a)] Normalization yields
\begin{align*}
1 &= \int_0^\infty \int_0^\infty f_{X, Y}(x, y) dx dy\\
&= \int_0^1 \int_0^{1 - y}  cx dx dy\\
&= \int_0^1 \frac{c}{2}(1 - y)^2 dy\\
&= \int_0^1 \frac{c}{2}(y^2 - 2y + 1) dy\\
&= \left. \frac{c}{2}(\frac{1}{3}y^3 - y^2 + y) \right|_0^1\\
&= \frac{c}{6}\\
c &= \boxed{6}.
\end{align*}
\item[(b)] In order to calculate $E(Y | X = x)$ and $E(X| Y = y)$, we will need to first find $f_{Y | X = x}(y)$ and $f_{X | Y = y}(x)$. To find these, we will first need to compute our marginal probability density functions. For $x \in [0, 1]$, we have
\begin{align*}
f_X(x) &= \int_{-\infty}^{\infty} f_{X, Y}(x, y) dy\\
&= \int_{0}^{1 - x} 6x dy\\
&=  6x(1 - x)
\end{align*}
Likewise, for $y \in [0, 1]$, we have
\begin{align*}
f_Y(y) &= \int_{-\infty}^{\infty} f_{X, Y}(x, y) dx\\
&= \int_{0}^{1 - y} 6x dx\\
&= 3(1 - y)^2.
\end{align*}
With this, we have
\begin{align*}
f_{X | Y = y}(x) &= \frac{f_{X, Y}(x, y)}{f_Y(y)}\\
&= \frac{6x}{3(1 - y)^2}\\
&= \frac{2x}{(1 - y)^2}
\end{align*}
and 
\begin{align*}
f_{Y | X = x}(y) &= \frac{f_{X, Y}(x, y)}{f_X(x)}\\
&= \frac{6x}{6x(1 - x)}\\
&= \frac{1}{1 - x},
\end{align*}
on the support of $f_{X, Y}(x, y)$. Finally, we have
\begin{align*}
E(X| Y = y) &= \int_{-\infty}^\infty xf_{X | Y = y}(x) dx\\
&= \int_{0}^{1 - y} \frac{2x^2}{(1 - y)^2} dx\\
&= \frac{2(1 - y)^3}{3(1 - y)^2}\\
&= \boxed{\frac{2}{3}(1 - y)},
\end{align*}
and 
\begin{align*}
E(Y| X = x) &= \int_{-\infty}^\infty yf_{Y | X = x}(y) dy\\
&= \int_{0}^{1 - x} \frac{y}{1 - x} dy\\
&= \frac{(1 - x)^2}{2(1 - x)}\\
&= \boxed{\frac{1}{2} (1 - x)}.
\end{align*}
\end{enumerate}

\section*{Problem 2.33}
Suppose that the random variable $X$ is uniformly distributed symmetrically around zero, but in such a way that the parameter is uniform on $(0, 1)$; that is suppose that
\begin{align*}
X|A = a \in U(-a, a) \text{ with } A \in U(0, 1).
\end{align*}
Find the distribution of $X$, $EX$, and Var$X$.

\subsection*{Solution}
We have
\begin{align*}
f_{X|A = a}(x) = \frac{f_{X, A}(x, a)}{f_A(a)} &\implies f_{X, A}(x, a) = f_{X|A = a}(x) \cdot f_A(a),
\end{align*}
thus
\begin{align*}
f_X(x) &= \int_{-\infty}^\infty f_{X, A}(x, a) da\\
&= \int_{-\infty}^\infty f_{X|A = a}(x) \cdot f_A(a) da.
\end{align*}
At this point, in order to correctly integrate over the support of $f_{X, A}(x, a)$, we will break this into case 1 where $-1 \leq x \leq 0$, and case 2 where $0 \leq x \leq 1$.
\begin{enumerate}
\item[(1)] Satisfying the conditions of our support, we have
\begin{align*}
f_X(x) &= \int_{-\infty}^\infty f_{X, A}(x, a) da\\
&= \int_{-x}^1 \frac{1}{2a} da\\
&= - \frac{1}{2} \ln (-x).
\end{align*}

\item[(2)] Satisfying the conditions of our support once more, we have
\begin{align*}
f_X(x) &= \int_{-\infty}^\infty f_{X, A}(x, a) da\\
&= \int_{x}^1 \frac{1}{2a} da\\
&= - \frac{1}{2} \ln (x).
\end{align*}
\end{enumerate}
We can succinctly write this as 
\begin{align*}
\boxed{f_X(x) = \frac{1}{2} \ln |x|},
\end{align*}
for $-1 \leq x \leq 1$.

Now, since we can see that $f_X(x)$ is even, we have that $xf_X(x)$ is odd, and we can automatically conclude that $\boxed{EX = 0}$. Thus, we have
\begin{align*}
\text{Var}X &= EX^2 - (EX)^2\\
&= EX^2.
\end{align*}
Now computing $EX^2$ directly with $f_X(x)$ requires some moderately difficult integration, so we will instead use our helper variable:
\begin{align*}
EX^2 &= E_{A}(E_{X|A = a}(X))\\
&= \int_0^1 f_A(a) \cdot (E_{X|A = a}(X)) da\\
&= \int_0^1 f_A(a) \cdot \left(\int_{-a}^a x^2 \cdot f_{X|A = a}(x) dx \right) da\\
&= \int_0^1 \int_{-a}^a \frac{x^2}{2a} dx da\\
&= \int_0^1 \int_{0}^a \frac{x^2}{a} dx da\\
&= \int_0^1 \frac{a^2}{3}da\\
&= \boxed{\frac{1}{9}}.
\end{align*}

\section*{Problem 2.34}
Consider the following model:
\begin{align*}
X_n | Y = y \in \text{Bin}(n, y) \text{ with } f_Y(y) = 6y(1-y), \text{ } 0 < y < 1.
\end{align*}
\begin{enumerate}
\item[(a)] Compute $EX_n$ and Var$X_n$.
\item[(b)] Determine the distribution of $X_n$.
\end{enumerate}

\subsection*{Solution}
\begin{enumerate}
\item[(a)] Since $X_n | Y = y \in \text{Bin}(n, y)$, we have
\begin{align*}
p_{X_n | Y = y}(k) &= {n \choose k} y^k (1 - y)^{n - k} \text{ for } k = 0, 1, ..., n.
\end{align*}
Thus, 
\begin{align*}
EX_n &= E_Y(E_{X_n|Y = y}(X_n))\\
&= \int_0^1 \left( \sum_{k = 0}^n  k \cdot p_{X_n | Y = y}(k)\right) \cdot f_Y(y) dy\\
&= \int_0^1 \left( \sum_{k = 0}^n k {n \choose k} y^k (1 - y)^{n - k} \right) 6y(1 - y) dy\\
&= \int_0^1 \left( \sum_{k = 0}^n  6k {n \choose k}  y^{k+1} (1 - y)^{n - k + 1} \right) dy\\
&= -\int_0^1 6n(y-1)y^2 dy \text{, found by entering into wolfram alpha} \\
&= -6n \int_0^1 (y^3 - y^2) dy\\
&= -6n(\frac{1}{4} - \frac{1}{3})\\
&= 6n(\frac{4}{12} - \frac{3}{12})\\
&= \boxed{\frac{n}{2}}.
\end{align*}
To find our variance, we compute $EX^2$ in a very similar manner
\begin{align*}
EX^2 &= \int_0^1 \left( \sum_{k = 0}^n  6k^2 {n \choose k}  y^{k+1} (1 - y)^{n - k + 1} \right) dy\\ 
&= -6 \int_0^1 (y-1)y^2((n-1)ny + n)dy\\
&= \frac{1}{10}n(3n + 2).
\end{align*}
Thus,
\begin{align*}
\text{Var}X &= EX^2 - (EX)^2\\
&= \frac{1}{10}n(3n + 2) - \left(\frac{n}{2}\right)^2\\
&= \boxed{\frac{n^2}{20} + \frac{n}{5}}
\end{align*}
\end{enumerate}

\section*{Problem 2.35}
Let $X$ and $Y$ be jointly distributed random variables such that $Y|X = x \in \text{Bin}(n, x)$ with $X \in U(0, 1)$. Compute $EY$, Var$Y$, and Cov$(X, Y)$.

\subsection*{Solution}
Similar to the previous problem, we know we have
\begin{align*}
p_{Y | X = x}(k) &= {n \choose k} x^k (1 - x)^{n - k} \text{ for } k = 0, 1, ..., n.
\end{align*}
We also have 
\begin{align*}
f_X(x) = \begin{cases} 
      1& 0 \leq x \leq \infty, \text{ and } 0 \leq x \leq 1 \\
      0 & \text{otherwise.}
   \end{cases}
\end{align*}

Similar to our previous problem, we have
\begin{align*}
E_Y &= E_{X}(E_{Y|X = x}(Y))\\
&= \int_0^1 \left(\sum_{k=0}^n  {n \choose k} k \cdot x^k (1 - x)^{n - k} \right) dx\\
&= \int_0^1 nx dx\\
&= \boxed{ \frac{n}{2}},
\end{align*}
and
\begin{align*}
EY^2 &= E_{X}(E_{Y|X = x}(Y^2))\\
&= \int_0^1 \left(\sum_{k=0}^n  {n \choose k} k^2 \cdot x^k (1 - x)^{n - k} \right) dx\\
&= \int_0^1 x (n + (-1 + n) n x) dx\\
&= \frac{1}{6} n (2n + 1)\\
&= \frac{n^2}{3} + \frac{n}{6}.
\end{align*}
Thus, we have
\begin{align*}
\text{Var}Y &= EY^2 - (EY)^2\\
&= \frac{n^2}{3} + \frac{n}{6} - \frac{n^2}{4}\\
&= \boxed{ \frac{n^2}{12} + \frac{n}{6}}.
\end{align*}
Finally, we have
\begin{align*}
\text{Cov}(X, Y) &= E((X - E(X))(Y - E(Y)))\\
&= \int_0^1 \sum_{k=0}^n (x - E(X))(k - E(Y))\cdot  p_{Y | X = x}(k) \cdot f_X(x) dx\\
&= \int_0^1 \sum_{k=0}^n \left(x - \frac{1}{2}\right)\left(k - \frac{n}{2}\right){n \choose k} x^k (1 - x)^{n - k} dx\\
&= \int_0^1 \frac{1}{4} n (1 - 2x)^2 dx && \text{Let u = 1 - 2x}\\
&= - \frac{1}{8} n \int_1^{-1} u^2 du\\
&=  \boxed{\frac{n}{12}}.
\end{align*}

\section*{Problem 2.37}
Let $X$ be the number of coin tosses until heads is obtained. Suppose that the probability of heads is unknown in the sense that we consider it to be a random variable $Y \in U(0, 1)$.
\begin{enumerate}
\item[(a)] Find the distribution of $X$.
\item[(b)] The expected value of an Fs-distributed random variable exists and is well known. What about $EX$?
\item[(c)] Suppose that the value $X = n$ has been observed. Find the posterior distribution of $Y$, that is, the distribution of $Y|X = n$.
\end{enumerate}

\subsection*{Solution}
\begin{enumerate}
\item[(a)] For $x = 1, 2, ...$, we have
\begin{align*}
p_X(x) &= \int_0^1 f_Y(y) \cdot p_{X|Y = y} dy\\
&= \int_0^1 (1 - y)^{x-1} y dy\\
&= \int_0^1 \frac{1}{x}(1 - y)^x dy && \text{Integration by parts}\\
&= \left. - \frac{1}{x(x+1)} (1 - y)^{x+1} \right|_0^1\\
&= \boxed{\frac{1}{x(x+1)}}.
\end{align*}
\item[(b)] We have
\begin{align*}
EX &= \sum_{x = 1}^\infty x p_X(x)\\
&= \sum_{x = 1}^\infty \frac{1}{x+1}.
\end{align*}
Employing the integral test, we see
\begin{align*}
\int_1^\infty \frac{1}{x+1} dx &= \left. ln(x + 1) \right|_1^\infty \to \infty,
\end{align*}
thus $EX$ does not exist.
\item[(c)] Finally, we have
\begin{align*}
f_{Y|X=n} &= \frac{f_{X, Y}(n, y)}{f_X(n)}\\
&= \frac{f_Y(y) \cdot f_{X|Y=y}(n)}{f_X(n)}\\
&= \boxed{(1-y)^{n - 1} y n(n + 1) \text{, for y = 1, 2, ...}}.
\end{align*}
\end{enumerate}

\end{document}